Finished the verification of the lookup in sequential bst via flow interface.

concurrency/verif_bst_flows.v
@@ -106,6 +106,56 @@ Proof.
       * rewrite <- Zgt_is_gt_bool. lia.
 Qed.
 
+Lemma split_left_dom: forall s e, e ∈ dom_ms s -> dom_ms (split_left s e) ⊂ dom_ms s.
+Proof.
+  intros. rewrite elem_of_subset. split.
+  - intros. rewrite nzmap_elem_of_dom in H0. destruct H0 as [a ?]. rewrite split_left_lookup in H0. destruct H0.
+    rewrite nzmap_elem_of_dom. exists a; easy.
+  - intro. specialize (H0 _ H). rewrite nzmap_elem_of_dom in H0. destruct H0. rewrite split_left_lookup in H0.
+    destruct H0. lia.
+Qed.
+
+Lemma split_right_dom: forall s e, e ∈ dom_ms s -> dom_ms (split_right s e) ⊂ dom_ms s.
+Proof.
+  intros. rewrite elem_of_subset. split.
+  - intros. rewrite nzmap_elem_of_dom in H0. destruct H0 as [a ?]. rewrite split_right_lookup in H0. destruct H0.
+    rewrite nzmap_elem_of_dom. exists a; easy.
+  - intro. specialize (H0 _ H). rewrite nzmap_elem_of_dom in H0. destruct H0. rewrite split_right_lookup in H0.
+    destruct H0. lia.
+Qed.
+
+Lemma split_left_dom_in: forall s e x, x ∈ dom_ms (split_left s e) -> x < e.
+Proof.
+  intros. rewrite nzmap_elem_of_dom in H. destruct H. rewrite split_left_lookup in H.
+  now destruct H.
+Qed.
+
+Lemma split_right_dom_in: forall s e x, x ∈ dom_ms (split_right s e) -> x > e.
+Proof.
+  intros. rewrite nzmap_elem_of_dom in H. destruct H. rewrite split_right_lookup in H.
+  now destruct H.
+Qed.
+
+Lemma split_left_right_dom_disjoint: forall s e, dom_ms (split_left s e) ∩ dom_ms (split_right s e) = ∅.
+Proof.
+  intros. rewrite <- disjoint_intersection_L. red. repeat intro.
+  rewrite nzmap_elem_of_dom in H. rewrite nzmap_elem_of_dom in H0.
+  destruct H as [a ?]. rewrite split_left_lookup in H. destruct H.
+  destruct H0 as [b ?]. rewrite split_right_lookup in H0. destruct H0. lia.
+Qed.
+
+Lemma split_left_not_in: forall s e, e ∉ dom_ms (split_left s e).
+Proof.
+  repeat intro. rewrite nzmap_elem_of_dom in H. destruct H. rewrite split_left_lookup in H.
+  destruct H. now apply Z.lt_irrefl in H0.
+Qed.
+
+Lemma split_right_not_in: forall s e, e ∉ dom_ms (split_right s e).
+Proof.
+  repeat intro. rewrite nzmap_elem_of_dom in H. destruct H. rewrite split_right_lookup in H.
+  destruct H. now apply Zgt_irrefl in H0.
+Qed.
+
 Definition inset_edgeFn (x y: TreeNode): K_multiset Z -> K_multiset Z :=
   fun s => if (val_eqb x.(addr_tn) y.(addr_tn) || val_eqb y.(addr_tn) nullval)%bool
            then ∅
@@ -193,12 +243,12 @@ Proof.
   now apply pc_tree_rep_saturate_local.
 Qed.
 
-Lemma tree_rep_neq_nullval: forall n l C1 C2,
-    In n l -> tree_rep l C1 C2 |-- !! (addr_tn n <> nullval).
+Lemma tree_rep_neq_nullval: forall l C1 C2,
+    tree_rep l C1 C2 |-- !! (forall n, In n l -> addr_tn n <> nullval).
 Proof.
-  intros. sep_apply tree_rep_impl_pc_tree_rep.
-  rewrite (pc_tree_rep_In_eq n); auto. Intros nI l' Cl.
-  unfold pc_node_rep. Intros. entailer !.
+  intros. eapply derives_trans. 2: apply allp_prop_left. apply allp_right. intros. rewrite prop_impl.
+  apply imp_andp_adjoint. Intros. sep_apply tree_rep_impl_pc_tree_rep.
+  rewrite (pc_tree_rep_In_eq v); auto. Intros nI l' Cl. unfold pc_node_rep. Intros. entailer !.
 Qed.
 
 Lemma tree_rep_cons: forall n l C1 C2,
@@ -323,8 +373,7 @@ Proof.
                                                               (left_tn p = addr_tn x ∨ right_tn p = addr_tn x)) y). {
     sep_apply Hit. sep_apply (tree_rep_has_unique_parent root); auto. entailer !. } rename H5 into Hunq.
   assert_PROP (forall n, In n l -> addr_tn n ≠ nullval). {
-    sep_apply Hit. eapply derives_trans. 2: apply allp_prop_left. apply allp_right. intros. rewrite prop_impl.
-    apply imp_andp_adjoint. Intros.  now apply tree_rep_neq_nullval. } rename H5 into Hnull.
+    sep_apply Hit. apply tree_rep_neq_nullval. } rename H5 into Hnull.
   assert_PROP (∀ x : TreeNode, In x l → left_tn x ≠ addr_tn root ∧ right_tn x ≠ addr_tn root). {
     sep_apply Hit. sep_apply (tree_rep_root_no_parent root); auto. entailer !. } rename H5 into Hrnp.
   assert_PROP (List.NoDup (map addr_tn l)). { sep_apply Hit. sep_apply tree_rep_nodup_addr. entailer !. }
@@ -332,7 +381,7 @@ Proof.
   destruct (Hloc _ H5). destruct (Hloc _ H6). destruct x as [x [xP xS]]. destruct y as [y [yP yS]].
   simpl fst in *. simpl snd in *. pose proof (in_combine_r _ _ _ _ H6). apply in_combine_r in H12.
   apply In_Permutation_cons in H12. destruct H12 as [fsl ?]. eapply list_join_perm in H2; eauto.
-  apply list_join_cons_inv in H2. destruct H2 as [Cl [? ?]]. red in H13.  
+  apply list_join_cons_inv in H2. destruct H2 as [Cl [? ?]]. red in H13.
   assert (x ≠ y) by (destruct H8 as [_ [? [? _]]]; intro; subst; destruct H7; exfalso; auto).
   pose proof (in_combine_r _ _ _ _ H5). apply in_combine_r in H15. eapply Permutation_in in H15; eauto.
   simpl in H15. destruct H15.
@@ -403,8 +452,7 @@ Proof.
                      node_rep x.1 x.2.1 x.2.2) (combine l (combine fpc fs)) |-- tree_rep l Cpc Cs). {
     unfold tree_rep. Exists fpc fs. entailer !. }
   assert_PROP (forall n, In n l -> addr_tn n ≠ nullval). {
-    sep_apply Hit. eapply derives_trans. 2: apply allp_prop_left. apply allp_right. intros. rewrite prop_impl.
-    apply imp_andp_adjoint. Intros.  now apply tree_rep_neq_nullval. } rename H5 into Hnull.
+    sep_apply Hit. apply tree_rep_neq_nullval. } rename H5 into Hnull.
   assert_PROP (∀ x : TreeNode, In x l → left_tn x = right_tn x ∧ left_tn x = nullval ∨ left_tn x ≠ right_tn x). {
     sep_apply Hit. sep_apply (tree_rep_left_right root); auto. entailer !. } rename H5 into Hlr.
   assert_PROP (List.NoDup (map addr_tn l)). { sep_apply Hit. sep_apply tree_rep_nodup_addr. entailer !. }
@@ -429,48 +477,313 @@ Proof.
       symmetry in H16. rewrite <- val_eqb_true in H16. now rewrite H16 in H13.
 Qed.
 
+Lemma tree_rep_inset_subset:
+  ∀ (root : TreeNode) (l : list TreeNode) (Cpc : pc_flowint) (Cs : bst_inset_flowint),
+    pc_global_inv root l Cpc → inset_global_inv root l Cs
+    → ∀ (fpc : list pc_flowint) (fs : list bst_inset_flowint),
+        list_join fpc Cpc → list_join fs Cs → length fpc = length l → length fs = length l
+        → iter_sepcon
+            (λ x : TreeNode * (pc_flowint * bst_inset_flowint),
+                node_rep x.1 x.2.1 x.2.2) (combine l (combine fpc fs))
+            |-- !! (∀ x y : TreeNode * (pc_flowint * bst_inset_flowint),
+                       In x (combine l (combine fpc fs)) → In y (combine l (combine fpc fs))
+                       -> left_tn x.1 = addr_tn y.1 \/ right_tn x.1 = addr_tn y.1 ->
+                       inset y.2.2 y.1 ⊂ inset x.2.2 x.1 /\
+                         ~ in_inset (key_tn x.1) y.2.2 y.1).
+Proof.
+  intros. assert (Hit: iter_sepcon
+                 (λ x : TreeNode * (pc_flowint * bst_inset_flowint),
+                     node_rep x.1 x.2.1 x.2.2) (combine l (combine fpc fs)) |-- tree_rep l Cpc Cs). {
+    unfold tree_rep. Exists fpc fs. entailer !. }
+  assert_PROP (forall x, In x l -> x ≠ root -> exists p, In p l /\ p ≠ x /\
+                                                           (left_tn p = addr_tn x ∨ right_tn p = addr_tn x)). {
+    sep_apply Hit. sep_apply (tree_rep_has_unique_parent root); auto. Intros. apply prop_right.
+    intros. specialize (H5 _ H6 H7). destruct H5 as [y [? ?]]. exists y; auto. } rename H5 into Huni.
+  sep_apply (tree_rep_inset_cnnt root l Cpc Cs). Intros. rename H5 into Hcnt.
+  sep_apply (tree_rep_inset_out root l Cpc Cs). Intros. rename H5 into Hout. sep_apply tree_rep_local_inv. Intros.
+  rename H5 into Hloc. apply prop_right. intros. specialize (Hcnt _ _ H5 H6 H7). specialize (Hout _ _ H5 H6).
+  destruct Hout. destruct x as [x [xP xS]]. destruct y as [y [yP yS]]. simpl fst in *. simpl snd in *.
+  unfold in_inset, inset. rewrite <- Hcnt. specialize (Hloc _ H5). destruct Hloc as [_ [_ [_ [? _]]]]. red in H10.
+  simpl in H10. destruct H7; [rewrite H8 | rewrite H9]; auto.
+  - split; [apply split_left_dom | apply split_left_not_in]; easy.
+  - split; [apply split_right_dom | apply split_right_not_in]; easy.
+Qed.
+
+Lemma perm_combine: forall {A B: Type} (l1: list A) (l2: list B) l,
+    combine l1 l2 ≡ₚ l -> exists p1 p2, l = combine p1 p2 /\ length l1 = length p1 /\ length l2 = length p2.
+Proof.
+  intros. remember (combine l1 l2) as l3. revert l1 l2 Heql3. induction H; intros.
+  - destruct l1.
+    + exists nil, l2. split; auto.
+    + destruct l2.
+      * exists (a :: l1), nil. split; auto.
+      * simpl in Heql3. inversion Heql3.
+  - rename Heql3 into H0. destruct l1. 1: simpl in H0; inversion H0. destruct l2.
+    1: rewrite combine_nil in H0; inversion H0. simpl in H0. inversion H0. apply IHPermutation in H3.
+    destruct H3 as [r1 [r2 [? [? ?]]]]. exists (a :: r1), (b :: r2). simpl. split; auto. f_equal; auto.
+  - rename Heql3 into H0. destruct l1. 1: simpl in H0; inversion H0. destruct l2.
+    1: rewrite combine_nil in H0; inversion H0. simpl in H0. inversion H0. subst. clear H0.
+    destruct l1. 1: simpl in H2; inversion H2. destruct l2. 1: rewrite combine_nil in H2; inversion H2. simpl in H2.
+    inversion H2. subst. exists (a0 :: a :: l1), (b0 :: b :: l2). now simpl.
+  - apply IHPermutation1 in Heql3. destruct Heql3 as [q1 [q2 [? [? ?]]]]. apply IHPermutation2 in H1.
+    destruct H1 as [p1 [p2 [? [? ?]]]]. exists p1, p2. split; auto. split; lia.
+Qed.
+
 Inductive ancestor: TreeNode -> TreeNode -> list TreeNode -> Prop :=
 | ancestor_parent: forall x, ancestor x x (x :: nil)
-| ancestor_more: forall x y z l, left_tn x = addr_tn z \/ right_tn x = addr_tn z ->
+| ancestor_more: forall x y z l, left_tn z = addr_tn x \/ right_tn z = addr_tn x ->
                                  ancestor z y l -> ancestor x y (x :: l).
+
+Lemma ancestor_sub: forall x y z l,
+    ancestor x y l -> In z l -> exists l1 l2, ancestor x z l1 /\ ancestor z y l2 /\ l = l1 ++ tl l2.
+Proof.
+  intros. revert x y z H H0. induction l; intros. 1: inversion H0. inversion H; subst; clear H; simpl in H0.
+  - destruct H0. 2: now exfalso. subst. exists [z], [z]. simpl tl. split; [|split]; constructor.
+  - destruct H0.
+    + subst. exists [z], (z :: l). simpl. split; [|split]; try constructor. apply ancestor_more with z0; auto.
+    + specialize (IHl _ _ _ H6 H). destruct IHl as [r1 [r2 [? [? ?]]]]. exists (a :: r1), r2. split; [|split]; auto.
+      * apply ancestor_more with z0; auto.
+      * rewrite <- app_comm_cons. now rewrite H2.
+Qed.
+
+Lemma ancestor_head: forall x y l, ancestor x y l -> head l = Some x. Proof. intros. inversion H; now simpl. Qed.
+
+Lemma ancestor_tail: forall x y l, ancestor x y l -> last l = Some y.
+Proof. intros. induction H; simpl; auto. rewrite last_cons. now rewrite IHancestor. Qed.
+
+Lemma ancestor_length: forall x y l, ancestor x y l -> (1 <= length l)%nat.
+Proof. intros. inversion H; simpl; lia. Qed.
+
+Lemma ancestor_snoc: forall x y l f,
+    ancestor x y (l ++ [f]) ->
+    f = y /\ (l = [] /\ x = y \/
+                (exists z, ancestor x z l /\ (left_tn y = addr_tn z \/ right_tn y = addr_tn z))).
+Proof.
+  intros. pose proof (ancestor_tail _ _ _ H). rewrite last_snoc in H0. inversion H0. subst. clear H0. split; auto.
+  remember (l ++ [y]). revert l Heql0. induction H; subst; intros.
+  - left. split; auto. symmetry. rewrite <- (app_inv_tail_iff [x]). now rewrite app_nil_l.
+  - right. destruct (nil_dec l). 1: subst l; inversion H0. apply exists_last in n. destruct n as [l1 [a ?H]].
+    rewrite H1 in Heql0. rewrite app_comm_cons in Heql0. apply app_inj_tail in Heql0. destruct Heql0. subst a.
+    specialize (IHancestor _ H1). destruct IHancestor as [[? ?] | [z0 [? ?]]].
+    + subst l1. subst l0. exists x. subst z. split; auto. constructor.
+    + exists z0. split; auto. subst l0. apply (ancestor_more x z0 z); auto.
+Qed.
+
+Lemma ancestor_head_in: forall x y l, ancestor x y l -> In x l.
+Proof. intros. induction H; simpl; left; easy. Qed.
+
+Lemma ancestor_tail_in: forall x y l, ancestor x y l -> In y l.
+Proof. intros. induction H; simpl; [left | right]; easy. Qed.
+
+Lemma incl_in_trans: forall {A: Type} x (l1 l2: list A), In x l1 -> incl l1 l2 -> In x l2.
+Proof. intros. now apply H0. Qed.
+
+Definition range_order (x: (TreeNode * (pc_flowint * bst_inset_flowint))) := size (inset x.2.2 x.1).
 
 Lemma tree_rep_root_for_all: forall root l Cpc Cs,
     !!(pc_global_inv root l Cpc /\ inset_global_inv root l Cs) &&
       tree_rep l Cpc Cs |--
-               !! (forall x, In x l -> exists sl, ancestor root x sl /\ incl sl l).
+               !! (forall x, In x l -> exists ! sl, ancestor x root sl /\ incl sl l).
 Proof.
   intros. Intros. sep_apply (tree_rep_has_unique_parent root); auto. Intros. rename H1 into Huni.
-  sep_apply tree_rep_nodup_addr. Intros. rename H1 into Hno.
-  assert_PROP (forall n, In n l -> addr_tn n ≠ nullval). {
-    eapply derives_trans. 2: apply allp_prop_left. apply allp_right. intros. rewrite prop_impl.
-    apply imp_andp_adjoint. Intros.  now apply tree_rep_neq_nullval. } rename H1 into Hnull.
-  sep_apply (tree_rep_left_right root); auto. Intros. rename H1 into Hlr. unfold tree_rep. Intros fpc fs.
-  sep_apply (tree_rep_inset_cnnt root l Cpc Cs). Intros. rename H5 into Hcnt.
-  sep_apply (tree_rep_inset_out root l Cpc Cs). Intros. rename H5 into Hout. sep_apply tree_rep_local_inv. Intros.
-  apply prop_right.
-  assert (forall x y, In x (combine l (combine fpc fs)) -> In y (combine l (combine fpc fs)) ->
-                      left_tn x.1 = addr_tn y.1 \/ right_tn x.1 = addr_tn y.1 ->
-                      inset y.2.2 y.1 ⊂ inset x.2.2 x.1). { admit. } intros. destruct (treenode_eq_dec x root).
-  - subst. exists (root :: nil). split. 1: constructor. destruct H as [? [? [? [? ?]]]].
-    repeat intro. simpl in H12. destruct H12; try easy. now subst.
-  -
-Abort.
+  sep_apply (tree_rep_root_no_parent root); auto. Intros. rename H1 into Hn.
+  unfold tree_rep. Intros fpc fs. sep_apply (tree_rep_inset_subset root l Cpc Cs). Intros.
+  remember (combine l (combine fpc fs)) as lc. remember (list_max (map range_order lc)) as maxS.
+  assert (forall x y, In x lc -> In y lc -> left_tn x.1 = addr_tn y.1 ∨ right_tn x.1 = addr_tn y.1 ->
+                      (maxS - range_order x < maxS - range_order y)%nat). {
+    intros. specialize (H5 _ _ H6 H7 H8). destruct H5 as [? _]. apply subset_size in H5. unfold range_order.
+    assert (forall z, In z lc -> range_order z <= maxS)%nat. {
+      assert (list_max (map range_order lc) <= maxS)%nat by lia. rewrite list_max_le in H9.
+      rewrite List.Forall_forall in H9. intros. apply (in_map range_order) in H10. now apply H9. }
+    apply H9 in H6, H7. unfold range_order in H6, H7. lia. } clear H5 HeqmaxS. rename H6 into Hr.
+  sep_apply tree_rep_local_inv. Intros. rename H5 into Hloc. apply prop_right.
+  intros. apply (In_fst_combine l (combine fpc fs)) in H5. 2: rewrite combine_length; lia. destruct H5.
+  rewrite <- Heqlc in H5. remember (maxS - range_order (x, x0))%nat as n. revert x x0 H5 Heqn.
+  induction n using lt_wf_ind; intros; subst. destruct (treenode_eq_dec x root).
+  - subst; exists (root :: nil); split; [split|]. 1: constructor.
+    + destruct H as [_ [_ [_ [? _]]]]. apply incl_cons; auto. apply incl_nil.
+    + intros ? [? ?]. inversion H7; clear H7; subst; auto. exfalso.
+      assert (In z l) by (apply ancestor_head_in in H10; apply H8; now right).
+      apply Hn in H7. destruct H7. now destruct H9.
+  - pose proof (in_combine_l _ _ _ _ H6). apply Huni in n; auto. destruct n as [? [[? [? Hp]] ?]].
+    apply (In_fst_combine l (combine fpc fs)) in H8. 2: rewrite combine_length; lia. destruct H8.
+    specialize (Hr _ _ H8 H6 Hp). edestruct H5 as [? [[? ?] ?]]; eauto.
+    eexists; split; [split|].
+    + eapply ancestor_more; eauto.
+    + intros ? [? | ?]; subst; auto.
+    + intros ? [? ?]. destruct x'. 1: inversion H14. pose proof (ancestor_head _ _ _ H14). simpl in H16.
+      inversion H16. subst t. clear H16. inversion H14; subst.
+      * exfalso. apply in_combine_l in H8. apply Hn in H8. destruct H8. now destruct Hp.
+      * apply incl_cons_inv in H15. destruct H15 as [? ?]. f_equal. apply H13; split; auto.
+        cut (z = x1). 1: intros; now subst. 
+        assert (In z l) by (apply ancestor_head_in in H20; now apply H16).
+        symmetry. apply H10. split; [|split]; auto. apply (In_fst_combine l (combine fpc fs)) in H18.
+        2: rewrite combine_length; lia. destruct H18. apply Hloc in H18. destruct H18 as [? _].
+        simpl in H18. destruct H18 as [? [? [? _]]]. intro. subst.
+        destruct H17; [apply H19 | apply H21]; easy.
+Qed.
+
+
+Lemma tree_rep_inset_disjoint:
+  ∀ (root : TreeNode) (l : list TreeNode) (Cpc : pc_flowint) (Cs : bst_inset_flowint),
+    pc_global_inv root l Cpc -> inset_global_inv root l Cs
+    -> ∀ (fpc : list pc_flowint) (fs : list bst_inset_flowint),
+        list_join fpc Cpc -> list_join fs Cs -> length fpc = length l -> length fs = length l
+        -> iter_sepcon
+            (λ x : TreeNode * (pc_flowint * bst_inset_flowint),
+                node_rep x.1 x.2.1 x.2.2) (combine l (combine fpc fs))
+            |-- !! (∀ x y z: TreeNode * (pc_flowint * bst_inset_flowint),
+                       In x (combine l (combine fpc fs)) ->
+                       In y (combine l (combine fpc fs)) ->
+                       In z (combine l (combine fpc fs)) ->
+                       left_tn x.1 = addr_tn y.1 ->
+                       right_tn x.1 = addr_tn z.1 ->
+                       inset y.2.2 y.1 ∩ inset z.2.2 z.1 = ∅).
+Proof.
+  intros. sep_apply (tree_rep_inset_cnnt root l Cpc Cs). Intros.
+  sep_apply (tree_rep_inset_out root l Cpc Cs). Intros.
+  apply prop_right. intros. pose proof (H5 _ _ H7 H8 (or_introl H10)). pose proof (H5 _ _ H7 H9 (or_intror H11)).
+  pose proof ((proj1 (H6 _ _ H7 H8)) H10). pose proof ((proj2 (H6 _ _ H7 H9)) H11). unfold inset.
+  rewrite <- H12, <- H13, H14, H15. apply split_left_right_dom_disjoint.
+Qed.
+
+Lemma NoDup_fst_impl_eq: forall {A B: Type} (l: list (A * B)) x y,
+    List.NoDup (map fst l) -> In x l -> In y l -> x.1 = y.1 -> x = y.
+Proof.
+  intros until l. induction l; intros. 1: inversion H0.
+  destruct H0, H1; simpl in H; rewrite NoDup_cons_iff in H; destruct H.
+  - subst; easy.
+  - subst. apply (in_map fst) in H1. now rewrite H2 in H.
+  - subst. apply (in_map fst) in H0. now rewrite H2 in H0.
+  - now apply IHl.
+Qed.
+
+Lemma tree_rep_ancestor_subset:
+  ∀ (root : TreeNode) (l : list TreeNode) (Cpc : pc_flowint) (Cs : bst_inset_flowint),
+    pc_global_inv root l Cpc → inset_global_inv root l Cs
+    → ∀ (fpc : list pc_flowint) (fs : list bst_inset_flowint),
+        list_join fpc Cpc → list_join fs Cs → length fpc = length l → length fs = length l
+        → iter_sepcon
+            (λ x : TreeNode * (pc_flowint * bst_inset_flowint),
+                node_rep x.1 x.2.1 x.2.2) (combine l (combine fpc fs))
+            |-- !! (∀ (x y : TreeNode * (pc_flowint * bst_inset_flowint)) sl,
+                       In x (combine l (combine fpc fs)) → In y (combine l (combine fpc fs))
+                       -> ancestor y.1 x.1 sl -> incl sl l -> inset y.2.2 y.1 ⊆ inset x.2.2 x.1).
+Proof.
+  intros. sep_apply (tree_rep_inset_subset root l Cpc Cs). Intros.
+  assert (Hit: iter_sepcon
+                 (λ x : TreeNode * (pc_flowint * bst_inset_flowint),
+                     node_rep x.1 x.2.1 x.2.2) (combine l (combine fpc fs)) |-- tree_rep l Cpc Cs). {
+    unfold tree_rep. Exists fpc fs. entailer !. }
+  assert_PROP (List.NoDup (map fst (combine l (combine fpc fs)))). {
+    rewrite combine_fst. 2: rewrite combine_length; lia. sep_apply Hit.
+    sep_apply tree_rep_nodup_addr. Intros. apply NoDup_map_inv in H6. entailer !. }
+  rename H6 into Hn. apply prop_right. intros.
+  revert sl x y H6 H7 H8 H9. induction sl; intros; inversion H8; subst.
+  - pose proof (NoDup_fst_impl_eq _ _ _ Hn H7 H6 H12). subst y. rewrite elem_of_subseteq. now intros.
+  - assert (In z l) by (apply ancestor_head_in in H15; apply H9; now right).
+    clear H8. apply (In_fst_combine l (combine fpc fs)) in H10. 2: rewrite combine_length; lia.
+    destruct H10 as [z2 ?]. specialize (H5 _ _ H8 H7 H14). specialize (IHsl _ _ H6 H8 H15).
+    assert (incl sl l). { unfold incl in *. intros. apply H9. now right. } specialize (IHsl H10).
+    simpl fst in *. simpl snd in *. destruct H5 as [[? ?] _]. transitivity (inset z2.2 z); auto.
+Qed.
 
 Lemma tree_rep_inset_range:
-  forall (l : list TreeNode) (Cpc : pc_flowint) (Cs : bst_inset_flowint)
-         (fpc : list pc_flowint) (fs : list bst_inset_flowint) root,
-    list_join fpc Cpc -> list_join fs Cs -> length fpc = length l ->
-    length fs = length l -> pc_global_inv root l Cpc ->
-    inset_global_inv root l Cs ->
-    (forall x, In x (combine l (combine fpc fs)) ->
-               pc_local_inv x.1 x.2.1 /\ inset_local_inv x.1 x.2.2) ->
-    forall x xI xS y yI yS z,
-      In (x, (xI, xS)) (combine l (combine fpc fs)) ->
-      In (y, (yI, yS)) (combine l (combine fpc fs)) -> x ≠ y ->
-      in_inset z xS x -> in_inset z yS y -> ancestor x y l \/ ancestor y x l.
+  ∀ (root : TreeNode) (l : list TreeNode) (Cpc : pc_flowint) (Cs : bst_inset_flowint),
+    pc_global_inv root l Cpc -> inset_global_inv root l Cs
+    -> ∀ (fpc : list pc_flowint) (fs : list bst_inset_flowint),
+        list_join fpc Cpc -> list_join fs Cs -> length fpc = length l -> length fs = length l
+        -> iter_sepcon
+            (λ x : TreeNode * (pc_flowint * bst_inset_flowint),
+                node_rep x.1 x.2.1 x.2.2) (combine l (combine fpc fs))
+            |-- !! (∀ (x y: TreeNode * (pc_flowint * bst_inset_flowint)) z,
+                       In x (combine l (combine fpc fs)) ->
+                       In y (combine l (combine fpc fs)) ->
+                       in_inset z x.2.2 x.1 -> in_inset z y.2.2 y.1 ->
+                       exists sl, incl sl l /\ (ancestor x.1 y.1 sl \/ ancestor y.1 x.1 sl)).
 Proof.
-  intros.
-Abort.
+  intros. sep_apply (tree_rep_inset_disjoint root l Cpc Cs). Intros. rename H5 into Hd.
+  sep_apply (tree_rep_ancestor_subset root l Cpc Cs). Intros. rename H5 into Hs.
+  assert (Hit: iter_sepcon
+                 (λ x : TreeNode * (pc_flowint * bst_inset_flowint),
+                     node_rep x.1 x.2.1 x.2.2) (combine l (combine fpc fs)) |-- tree_rep l Cpc Cs). {
+    unfold tree_rep. Exists fpc fs. entailer !. }
+  assert_PROP (List.NoDup (map addr_tn l)) by (sep_apply Hit; apply tree_rep_nodup_addr). rename H5 into Hn.
+  assert_PROP (forall x, In x l -> exists ! sl, ancestor x root sl /\ incl sl l). {
+    sep_apply Hit. sep_apply (tree_rep_root_for_all root l Cpc Cs); auto. Intros. now apply prop_right. }
+  clear Hit. rename H5 into Hr. apply prop_right. intros. destruct x as [x [xP xS]]. destruct y as [y [yP yS]].
+  simpl fst in *. simpl snd in *. destruct (Hr _ (in_combine_l _ _ _ _ H5)) as [xl [[? ?] _]].
+  destruct (Hr _ (in_combine_l _ _ _ _ H6)) as [yl [[? ?] _]].
+  assert (forall m, In m l -> exists mp, In (m, mp) (combine l (combine fpc fs))). {
+    intros; apply In_fst_combine; auto. rewrite combine_length; lia. } rename H13 into Hc.
+  destruct (le_ge_dec (length xl) (length yl)).
+  - assert (exists zl, yl = zl ++ xl). {
+      clear H H0 Hr. revert dependent root. revert dependent yl. revert dependent xl.
+      apply (rev_ind (fun xl => incl xl l
+                                → ∀ yl : list TreeNode,
+                          incl yl l → (length xl <= length yl)%nat →
+                          ∀ root : TreeNode, ancestor x root xl → ancestor y root yl →
+                                             ∃ zl : list TreeNode, yl = zl ++ xl)); intros. 1: inversion H10.
+      rewrite last_length in H10. rename l0 into xl. assert (yl ≠ []) by (destruct yl; auto; simpl in H10; lia).
+      destruct (exists_last H13) as [l1 [y0 ?]]. subst yl. clear H13. rewrite last_length in H10. rename l1 into yl.
+      apply le_S_n in H10. apply ancestor_snoc in H11. apply ancestor_snoc in H12. destruct H11, H12. subst x0 y0.
+      apply incl_app_inv in H0, H9. destruct H13 as [[? ?] | [zx [? ?]]]. 1: subst; exists yl; f_equal.
+      destruct H14 as [[? ?] | [zy [? ?]]]. 1: exfalso; subst yl; apply ancestor_length in H11; simpl in H10; lia.
+      pose proof (ancestor_tail_in _ _ _ H11). pose proof (ancestor_tail_in _ _ _ H13). apply H0 in H15.
+      apply H9 in H16. destruct H12, H14.
+      - rewrite H12 in H14. pose proof (map_nodup_neq_nodup _ _ _ _ Hn H15 H16 H14). subst zy.
+        specialize (H (proj1 H0) _ (proj1 H9) H10 _ H11 H13).
+        destruct H as [zl ?]. exists zl. subst. now rewrite app_assoc.
+      - assert (In root l) by (apply H0; now left). apply Hc in H15, H16, H17. destruct H15, H16, H17.
+        specialize (Hd _ _ _ H17 H15 H16 H12 H14). simpl in Hd. exfalso.
+        pose proof (Hs _ _ _ H15 H5 H11 (proj1 H0)). pose proof (Hs _ _ _ H16 H6 H13 (proj1 H9)). simpl in H18, H19.
+        rewrite <- disjoint_intersection_L in Hd. hnf in Hd. rewrite elem_of_subseteq in H18.
+        rewrite elem_of_subseteq in H19. now specialize (Hd _ (H18 _ H7) (H19 _ H8)).
+      - assert (In root l) by (apply H0; now left). apply Hc in H15, H16, H17. destruct H15, H16, H17.
+        specialize (Hd _ _ _ H17 H16 H15 H14 H12). simpl in Hd. exfalso.
+        pose proof (Hs _ _ _ H15 H5 H11 (proj1 H0)). pose proof (Hs _ _ _ H16 H6 H13 (proj1 H9)). simpl in H18, H19.
+        rewrite <- disjoint_intersection_L in Hd. hnf in Hd. rewrite elem_of_subseteq in H18.
+        rewrite elem_of_subseteq in H19. now specialize (Hd _ (H19 _ H8) (H18 _ H7)).
+      - rewrite H12 in H14. pose proof (map_nodup_neq_nodup _ _ _ _ Hn H15 H16 H14). subst zy.
+        specialize (H (proj1 H0) _ (proj1 H9) H10 _ H11 H13).
+        destruct H as [zl ?]. exists zl. subst. now rewrite app_assoc. } destruct H13 as [zl ?].
+    assert (In x yl) by (subst yl; rewrite in_app; right; now apply ancestor_head_in in H9).
+    destruct (ancestor_sub _ _ _ _ H11 H14) as [l1 [l2 [? [? ?]]]]. exists l1. split; auto.
+    clear H13. subst yl. apply incl_app_inv in H12. now destruct H12.
+  - unfold ge in g. assert (exists zl, xl = zl ++ yl). {
+      clear H H0 Hr. revert dependent root. revert dependent xl. revert dependent yl.
+      apply (rev_ind (fun yl => incl yl l
+                                → ∀ xl : list TreeNode,
+                          incl xl l → (length yl <= length xl)%nat →
+                          ∀ root : TreeNode, ancestor x root xl → ancestor y root yl →
+                                             ∃ zl : list TreeNode, xl = zl ++ yl)); intros. 1: inversion H11.
+      rewrite last_length in H10. rename l0 into yl. assert (xl ≠ []) by (destruct xl; auto; simpl in H10; lia).
+      destruct (exists_last H13) as [l1 [y0 ?]]. subst xl. clear H13. rewrite last_length in H10. rename l1 into xl.
+      apply le_S_n in H10. apply ancestor_snoc in H11. apply ancestor_snoc in H12. destruct H11, H12. subst x0 y0.
+      apply incl_app_inv in H0, H9. destruct H14 as [[? ?] | [zy [? ?]]]. 1: subst; exists xl; f_equal.
+      destruct H13 as [[? ?] | [zx [? ?]]]. 1: exfalso; subst xl; apply ancestor_length in H11; simpl in H10; lia.
+      pose proof (ancestor_tail_in _ _ _ H11). pose proof (ancestor_tail_in _ _ _ H13). apply H0 in H15.
+      apply H9 in H16. destruct H12, H14.
+      - rewrite H12 in H14. pose proof (map_nodup_neq_nodup _ _ _ _ Hn H15 H16 H14). subst zy.
+        specialize (H (proj1 H0) _ (proj1 H9) H10 _ H13 H11).
+        destruct H as [zl ?]. exists zl. subst. now rewrite app_assoc.
+      - assert (In root l) by (apply H0; now left). apply Hc in H15, H16, H17. destruct H15, H16, H17.
+        specialize (Hd _ _ _ H17 H15 H16 H12 H14). simpl in Hd. exfalso.
+        pose proof (Hs _ _ _ H15 H6 H11 (proj1 H0)). pose proof (Hs _ _ _ H16 H5 H13 (proj1 H9)). simpl in H18, H19.
+        rewrite <- disjoint_intersection_L in Hd. hnf in Hd. rewrite elem_of_subseteq in H18.
+        rewrite elem_of_subseteq in H19. now specialize (Hd _ (H18 _ H8) (H19 _ H7)).
+      - assert (In root l) by (apply H0; now left). apply Hc in H15, H16, H17. destruct H15, H16, H17.
+        specialize (Hd _ _ _ H17 H16 H15 H14 H12). simpl in Hd. exfalso.
+        pose proof (Hs _ _ _ H15 H6 H11 (proj1 H0)). pose proof (Hs _ _ _ H16 H5 H13 (proj1 H9)). simpl in H18, H19.
+        rewrite <- disjoint_intersection_L in Hd. hnf in Hd. rewrite elem_of_subseteq in H18.
+        rewrite elem_of_subseteq in H19. now specialize (Hd _ (H19 _ H7) (H18 _ H8)).
+      - rewrite H12 in H14. pose proof (map_nodup_neq_nodup _ _ _ _ Hn H15 H16 H14). subst zy.
+        specialize (H (proj1 H0) _ (proj1 H9) H10 _ H13 H11).
+        destruct H as [zl ?]. exists zl. subst. now rewrite app_assoc. } destruct H13 as [zl ?].
+    assert (In y xl) by (subst xl; rewrite in_app; right; now apply ancestor_head_in in H11).
+    destruct (ancestor_sub _ _ _ _ H9 H14) as [l1 [l2 [? [? ?]]]]. exists l1. split; auto.
+    clear H13. subst xl. apply incl_app_inv in H10. now destruct H10.
+Qed.
 
 Definition lookup_inv (root: TreeNode) (b: val) (l: list TreeNode)
            (Cpc : pc_flowint) (Cs: bst_inset_flowint) (x: Z): environ -> mpred :=
@@ -486,7 +799,6 @@ Definition lookup_inv (root: TreeNode) (b: val) (l: list TreeNode)
                           if Val.eq (addr_tn n) nullval then emp else node_rep n nI nS;
                           tree_rep l' Cl Cls).
 
-
 Lemma body_lookup: semax_body Vprog Gprog f_lookup lookup_spec.
 Proof.
   start_function.
@@ -494,12 +806,12 @@ Proof.
   Intros. sep_apply (tree_rep_root_no_parent root); auto. Intros. rename H4 into Hr.
   sep_apply tree_rep_nodup_addr. Intros. rename H4 into Hno.
   sep_apply (tree_rep_has_unique_parent root); auto. Intros. rename H4 into Huni.
-  sep_apply (tree_rep_left_right root); auto. Intros. rename H4 into Hlr. forward.
+  sep_apply (tree_rep_left_right root); auto. Intros. rename H4 into Hlr.
+  sep_apply (tree_rep_neq_nullval); Intros. rename H4 into Hnull. forward.
   - entailer. sep_apply (tree_rep_saturate_local root l Cpc Cs); auto. entailer !.
   - forward_while (lookup_inv root b l Cpc Cs x).
     + Exists root. destruct H1 as [_ [_ [_ [? _]]]].
-      sep_apply (tree_rep_neq_nullval root l Cpc Cs). Intros.
-      rewrite (tree_rep_In_eq root l Cpc Cs H1). Intros nI nS l' Cl1 Cl2.
+      pose proof (Hnull root H1). rewrite (tree_rep_In_eq root l Cpc Cs H1). Intros nI nS l' Cl1 Cl2.
       Exists l' nI Cl1 nS Cl2. if_tac. 1: now exfalso.
       assert_PROP (root ∈ domm nS). {
         unfold node_rep. Intros. apply prop_right. destruct H9 as [_ [? _]].
@@ -521,21 +833,70 @@ Proof.
         -- rewrite H3. entailer !.
         -- sep_apply H12. rewrite H16. sep_apply (tree_rep_is_ptr_null p l Cpc Cs). entailer !.
         -- Exists (empty_node, l, ∅ : pc_flowint, Cpc, ∅ : bst_inset_flowint, Cs). simpl fst. simpl snd.
-           if_tac. 2: cbn in H15; now exfalso. clear H15. entailer. apply andp_right. 2: sep_apply H12; entailer !.
-           unfold tree_rep. Intros fpc fs. sep_apply tree_rep_local_inv. Intros. apply prop_right.
+           if_tac. 2: cbn in H15; now exfalso. clear H15. unfold tree_rep at 1. Intros fpc fs.
+           symmetry in H10. pose proof (pc_global_inv_perm _ _ _ _ H10 H1).
+           pose proof (inset_global_inv_perm _ _ _ _ H10 H2).
+           assert (list_join (nI :: fpc) Cpc) by (apply join_cons with Cl; auto).
+           assert (list_join (nS :: fs) Cs) by (apply join_cons with Cls; auto).
+           assert (length (nI :: fpc) = length (n :: l')) by (simpl; auto).
+           assert (length (nS :: fs) = length (n :: l')) by (simpl; auto).
+           gather_SEP (iter_sepcon _ _) (data_at Tsh t_struct_tree _ (addr_tn n)).
+           replace_SEP 0 (iter_sepcon (λ y, node_rep y.1 y.2.1 y.2.2)
+                                      (combine (n :: l') (combine (nI :: fpc) (nS :: fs)))). {
+            entailer !. simpl combine. simpl iter_sepcon. cancel. unfold node_rep. entailer!. }
+          sep_apply (tree_rep_inset_range root (n :: l') Cpc Cs); Intros. rename H25 into Hanc.
+           sep_apply (tree_rep_inset_cnnt root (n :: l') Cpc Cs); Intros. rename H25 into Hcnnt.
+           sep_apply (tree_rep_inset_out root (n :: l') Cpc Cs); Intros. rename H25 into Hout.
+           sep_apply (tree_rep_ancestor_subset root (n :: l') Cpc Cs); Intros. rename H25 into Hset.
+           sep_apply (tree_rep_inset_subset root (n :: l') Cpc Cs); Intros. rename H25 into Hsub.
+           entailer. apply andp_right.
+           2: { simpl iter_sepcon. unfold node_rep at 1. Intros. cancel.
+                rewrite (tree_rep_In_eq n l Cpc Cs); auto. Exists nI nS l' Cl Cls.
+                unfold tree_rep. unfold node_rep at 2. symmetry in H10. entailer !. Exists fpc fs. entailer!. }
+           sep_apply tree_rep_local_inv. Intros. rename H28 into Hl. apply prop_right.
            split; [|split]; [apply intJoin_left_unit..|]. destruct H9 as [? [? [? [? [? [? [? ?]]]]]]].
            rewrite Int.signed_repr in H14; auto.
-        (* if the key was in some other node, then it would be removed from
-           the inset of all that node's descendants, contradicting the assumption
-           that it’s in the inset of a leaf node.  *)
-           intro. apply list_in_map_inv in H32. destruct H32 as [xN [? ?]].
-           assert (In xN l'). {
-            symmetry in H10. apply (Permutation_in xN H10) in H33. destruct H33; auto. subst. lia. }
-          admit.
+           (*  if the key was in some other node, then it would be removed from *)
+           (* the inset of all that node's descendants, contradicting the assumption *)
+           (* that it’s in the inset of a leaf node. *)
+           intro. apply list_in_map_inv in H35. destruct H35 as [xN [? ?]].
+           apply (Permutation_in xN H10) in H36.
+           assert (In (n, (nI, nS)) (combine (n :: l') (combine (nI :: fpc) (nS :: fs)))) by
+             (simpl; now left). apply (In_fst_combine _ (combine (nI :: fpc) (nS :: fs))) in H36.
+           2: rewrite combine_length; lia. destruct H36 as [xNR ?].
+           destruct (Hl _ H36) as [_ [_ [_ [? _]]]]. simpl in H38. rewrite <- H35 in H38.
+           specialize (Hanc _ _ x H36 H37 H38 H6). simpl in Hanc. destruct Hanc as [sl [? ?]].
+           destruct H40.
+           ++ assert (sl ≠ []) by (inversion H40; auto). apply exists_last in H41.
+              destruct H41 as [l1 [a ?]]. subst sl. apply ancestor_snoc in H40.
+              destruct H40 as [? [[? ?] | ?]]. 1: subst xN; lia. destruct H41 as [z [? ?]].
+              assert (In z (n :: l')). {
+               apply ancestor_tail_in in H41. apply incl_app_inv in H39. now apply H39 in H41. }
+             pose proof H43. apply (In_fst_combine _ (combine (nI :: fpc) (nS :: fs))) in H44.
+              2: rewrite combine_length; lia. destruct H44 as [zR ?].
+              specialize (Hcnnt _ _ H37 H44 H42). simpl in Hcnnt.
+              specialize (Hout _ _ H37 H44). destruct Hout as [_ ?]. destruct H42.
+              ** rewrite H42 in H3. symmetry in H10. apply (Permutation_in z H10) in H43.
+                 apply Hnull in H43. auto.
+              ** specialize (H45 H42). simpl in H45. rewrite Hcnnt in H45.
+                 apply incl_app_inv in H39. specialize (Hset _ _ _ H44 H36 H41 (proj1 H39)).
+                 simpl in Hset. rewrite elem_of_subseteq in Hset. specialize (Hset _ H38).
+                 unfold inset in Hset. rewrite H45 in Hset. apply split_right_dom_in in Hset. lia.
+           ++ assert (sl ≠ []) by (inversion H40; auto). apply exists_last in H41.
+              destruct H41 as [l1 [a ?]]. subst sl. apply ancestor_snoc in H40.
+              destruct H40 as [? [[? ?] | ?]]. 1: subst n; lia. destruct H41 as [z [? ?]].
+              assert (In z (n :: l')). {
+               apply ancestor_tail_in in H41. apply incl_app_inv in H39. now apply H39 in H41. }
+             apply (In_fst_combine _ (combine (nI :: fpc) (nS :: fs))) in H43.
+              2: rewrite combine_length; lia. destruct H43 as [zR ?]. apply incl_app_inv in H39.
+              specialize (Hsub _ _ H36 H43 H42). simpl in Hsub. destruct Hsub as [_ ?].
+              specialize (Hset _ _ _ H43 H37 H41 (proj1 H39)). simpl in Hset.
+              rewrite elem_of_subseteq in Hset. specialize (Hset _ H6). apply H44. now rewrite <- H35.
         -- rewrite H16. assert (In p l'). {
             symmetry in H10. apply Permutation_in with (l' := n :: l') in H3; auto.
             simpl in H3. destruct H3; auto. symmetry in H3. now exfalso. }
-          sep_apply (tree_rep_neq_nullval p l' Cl Cls). Intros.
+          assert (addr_tn p ≠ nullval). {
+            apply Hnull. eapply Permutation_in; eauto. now right. }
            rewrite (tree_rep_In_eq p l' Cl Cls); auto. Intros pI pS pl pClpc pCls.
            apply intJoin_comm in H4, H5. destruct (intJoin_assoc _ _ _ _ _ H19 H4) as [pIpc [? ?]].
            destruct (intJoin_assoc _ _ _ _ _ H20 H5) as [pSs [? ?]].
@@ -571,15 +932,76 @@ Proof.
         -- forward; destruct H13 as [? | [p [? [? ?]]]].
            ++ rewrite H13; entailer !.
            ++ sep_apply H12. rewrite H17. sep_apply (tree_rep_is_ptr_null p l Cpc Cs). entailer !.
-           ++ admit.
+           ++ Exists (empty_node, l, ∅ : pc_flowint, Cpc, ∅ : bst_inset_flowint, Cs). simpl fst.
+              simpl snd. if_tac. 2: cbn in H16; now exfalso. clear H16.
+              unfold tree_rep at 1. Intros fpc fs. symmetry in H10.
+              pose proof (pc_global_inv_perm _ _ _ _ H10 H1).
+              pose proof (inset_global_inv_perm _ _ _ _ H10 H2).
+              assert (list_join (nI :: fpc) Cpc) by (apply join_cons with Cl; auto).
+              assert (list_join (nS :: fs) Cs) by (apply join_cons with Cls; auto).
+              assert (length (nI :: fpc) = length (n :: l')) by (simpl; auto).
+              assert (length (nS :: fs) = length (n :: l')) by (simpl; auto).
+              gather_SEP (iter_sepcon _ _) (data_at Tsh t_struct_tree _ (addr_tn n)).
+              replace_SEP 0 (iter_sepcon (λ y, node_rep y.1 y.2.1 y.2.2)
+                                         (combine (n :: l') (combine (nI :: fpc) (nS :: fs)))). {
+               entailer !. simpl combine. simpl iter_sepcon. cancel. unfold node_rep. entailer!. }
+             sep_apply (tree_rep_inset_range root (n :: l') Cpc Cs); Intros. rename H26 into Hanc.
+              sep_apply (tree_rep_inset_cnnt root (n :: l') Cpc Cs); Intros. rename H26 into Hcnnt.
+              sep_apply (tree_rep_inset_out root (n :: l') Cpc Cs); Intros. rename H26 into Hout.
+              sep_apply (tree_rep_ancestor_subset root (n :: l') Cpc Cs); Intros. rename H26 into Hset.
+              sep_apply (tree_rep_inset_subset root (n :: l') Cpc Cs); Intros. rename H26 into Hsub.
+              entailer. apply andp_right.
+              2: { simpl iter_sepcon. unfold node_rep at 1. Intros. cancel.
+                   rewrite (tree_rep_In_eq n l Cpc Cs); auto. Exists nI nS l' Cl Cls.
+                   unfold tree_rep. unfold node_rep at 2. symmetry in H10. entailer !.
+                   Exists fpc fs. entailer!. }
+              sep_apply tree_rep_local_inv. clear H28. Intros. rename H28 into Hl. apply prop_right.
+              split; [|split]; [apply intJoin_left_unit..|].
+              destruct H9 as [? [? [? [? [? [? [? ?]]]]]]]. rewrite Int.signed_repr in H15; auto.
+              intro. apply list_in_map_inv in H35. destruct H35 as [xN [? ?]].
+              apply (Permutation_in xN H10) in H36.
+              assert (In (n, (nI, nS)) (combine (n :: l') (combine (nI :: fpc) (nS :: fs)))) by
+                (simpl; now left). apply (In_fst_combine _ (combine (nI :: fpc) (nS :: fs))) in H36.
+              2: rewrite combine_length; lia. destruct H36 as [xNR ?].
+              destruct (Hl _ H36) as [_ [_ [_ [? _]]]]. simpl in H38. rewrite <- H35 in H38.
+              specialize (Hanc _ _ x H36 H37 H38 H6). simpl in Hanc. destruct Hanc as [sl [? ?]].
+              destruct H40.
+              ** assert (sl ≠ []) by (inversion H40; auto). apply exists_last in H41.
+                 destruct H41 as [l1 [a ?]]. subst sl. apply ancestor_snoc in H40.
+                 destruct H40 as [? [[? ?] | ?]]. 1: subst xN; lia. destruct H41 as [z [? ?]].
+                 assert (In z (n :: l')). {
+                  apply ancestor_tail_in in H41. apply incl_app_inv in H39. now apply H39 in H41. }
+                pose proof H43. apply (In_fst_combine _ (combine (nI :: fpc) (nS :: fs))) in H44.
+                 2: rewrite combine_length; lia. destruct H44 as [zR ?].
+                 specialize (Hcnnt _ _ H37 H44 H42). simpl in Hcnnt.
+                 specialize (Hout _ _ H37 H44). destruct Hout as [? _]. destruct H42.
+                 --- specialize (H45 H42). simpl in H45. rewrite Hcnnt in H45.
+                     apply incl_app_inv in H39. specialize (Hset _ _ _ H44 H36 H41 (proj1 H39)).
+                     simpl in Hset. rewrite elem_of_subseteq in Hset. specialize (Hset _ H38).
+                     unfold inset in Hset. rewrite H45 in Hset. apply split_left_dom_in in Hset. lia.
+                 --- rewrite H42 in H13. symmetry in H10. apply (Permutation_in z H10) in H43.
+                     apply Hnull in H43. auto.
+              ** assert (sl ≠ []) by (inversion H40; auto). apply exists_last in H41.
+                 destruct H41 as [l1 [a ?]]. subst sl. apply ancestor_snoc in H40.
+                 destruct H40 as [? [[? ?] | ?]]. 1: subst n; lia. destruct H41 as [z [? ?]].
+                 assert (In z (n :: l')). {
+                  apply ancestor_tail_in in H41. apply incl_app_inv in H39. now apply H39 in H41. }
+                apply (In_fst_combine _ (combine (nI :: fpc) (nS :: fs))) in H43.
+                 2: rewrite combine_length; lia. destruct H43 as [zR ?]. apply incl_app_inv in H39.
+                 specialize (Hsub _ _ H36 H43 H42). simpl in Hsub. destruct Hsub as [_ ?].
+                 specialize (Hset _ _ _ H43 H37 H41 (proj1 H39)). simpl in Hset.
+                 rewrite elem_of_subseteq in Hset. specialize (Hset _ H6). apply H44.
+                 now rewrite <- H35.
            ++ rewrite H17. assert (In p l'). {
                symmetry in H10. apply Permutation_in with (l' := n :: l') in H13; auto.
                simpl in H13. destruct H13; auto. symmetry in H13. now exfalso. }
-             sep_apply (tree_rep_neq_nullval p l' Cl Cls). Intros.
+             assert (addr_tn p ≠ nullval). {
+               apply Hnull. eapply Permutation_in; eauto. now right. }
               rewrite (tree_rep_In_eq p l' Cl Cls); auto. Intros pI pS pl pClpc pCls.
               apply intJoin_comm in H4, H5. destruct (intJoin_assoc _ _ _ _ _ H20 H4) as [pIpc [? ?]].
-              destruct (intJoin_assoc _ _ _ _ _ H21 H5) as [pSs [? ?]]. Exists (p, (n :: pl), pI, pIpc, pS, pSs).
-              simpl fst. simpl snd. if_tac. 1: now exfalso. unfold tree_rep at 1. Intros fpc fs.
+              destruct (intJoin_assoc _ _ _ _ _ H21 H5) as [pSs [? ?]].
+              Exists (p, (n :: pl), pI, pIpc, pS, pSs). simpl fst. simpl snd. if_tac.
+              1: now exfalso. unfold tree_rep at 1. Intros fpc fs.
               sep_apply tree_rep_local_inv. Intros.
               gather_SEP (iter_sepcon _ _) (node_rep _ _ _) (data_at Tsh t_struct_tree _ (addr_tn n)).
               replace_SEP 0 (iter_sepcon (λ y, node_rep y.1 y.2.1 y.2.2)
@@ -615,4 +1037,4 @@ Proof.
     + if_tac. 2: now exfalso. forward. Exists nullval.
       destruct H6 as [? [? [? [? [? ?]]]]]. entailer !. unfold treebox_rep.
       entailer !.
-Abort.
+Qed.
